\[ \begin{aligned}
M(\theta) &= \mathcal{A}^T \mathcal{L}^T(\theta) \mathcal{G} \mathcal{L}(\theta) \mathcal{A}, \\
\dot{\theta} &= 0 \\
c(\theta, \dot{\theta}) &= -\mathcal{A}^T \mathcal{L}^T(\theta) \left( \mathcal{G} \mathcal{L}(\theta) \left[ \text{ad}_{\mathcal{A} \dot{\theta}} \right] \mathcal{W}(\theta) + \left[ \text{ad}_{\mathcal{V}} \right]^T \mathcal{G} \right) \mathcal{L}(\theta) \mathcal{A} \dot{\theta} \\
g(\theta) &= \mathcal{A}^T \mathcal{L}^T(\theta) \mathcal{g} \mathcal{L}(\theta) \dot{\mathcal{V}}_{\text{base}}
\end{aligned} \]
